src/parser/desugar.fs
@@ -74,10 +74,10 @@ let op_as_tylid r s =
     | "~"   ->  r Const.not_lid
     | "=="  ->  r Const.eq2_lid
     | "=!=" ->  r Const.neq2_lid
-    | "<" ->    r Const.lt_lid
-    | "<=" ->   r Const.lte_lid
-    | ">" ->    r Const.gt_lid
-    | ">=" ->   r Const.gte_lid
+//    | "<" ->    r Const.lt_lid
+//    | "<=" ->   r Const.lte_lid
+//    | ">" ->    r Const.gt_lid
+//    | ">=" ->   r Const.gte_lid
     | "/\\" ->  r Const.and_lid
     | "\\/" ->  r Const.or_lid
     | "==>" ->  r Const.imp_lid
@@ -97,10 +97,10 @@ let rec is_type env (t:term) =
     | Op("\\/", _)
     | Op("==>", _)
     | Op("<==>", _)  -> true               (* negation predicate *)
-    | Op("<", _)
-    | Op("<=", _)
-    | Op(">", _)
-    | Op(">=", _) -> env.phase = Formula
+//    | Op("<", _)
+//    | Op("<=", _)
+//    | Op(">", _)
+//    | Op(">=", _) -> env.phase = Formula
     | Op(s, _) -> (match op_as_tylid t.range s with
         | None -> false
         | _ -> true)
