examples/unit-tests/stlc.fst
@@ -72,16 +72,8 @@ type env = int -> Tot (option ty)
 val empty : env
 let empty _ = None
 
-(* CH: This should work but it seems that F* stumbles upon the type abbreviation
 val extend : env -> int -> ty -> Tot env
-let extend g x t  = (fun x' -> if x = x' then Some t else g x')
-   Now it stumbles a bit later below:
-bug23.fst(8,31-8,32) : Error
-Too many arguments to function of type (_:env -> _:int -> _:ty -> Tot env)
-*)
-
-val extend : env -> int -> ty -> int -> Tot (option ty)
-let extend g x t  = (fun x' -> if x = x' then Some t else g x')
+let extend g x t x' = if x = x' then Some t else g x'
 
 let x45 = extend (extend empty 42 TBool) 0 (TArrow TBool TBool)
 
@@ -117,41 +109,21 @@ let rec typing e g =
       | Some TBool, Some t2, Some t3 -> if t2 = t3 then Some t2 else None
       | _         , _      , _       -> None
        end
-  | _ -> None
 
-(* This proof should really be trivial (see canonical_forms_fun below) *)
 val canonical_forms_bool : e:exp -> Pure unit
-      (requires ((typing e empty = Some TBool) /\ (is_value e = true)))
-      (ensures \r -> (e = ETrue) \/ (e = EFalse))
-let canonical_forms_bool e = 
-  match e with
-  | EVar x -> ()
-  | EAbs x' t e1 -> admit() //NS: fishy ...invetigating
-  | EApp e1 e2 -> ()
-  | ETrue -> ()
-  | EFalse -> ()
-  | EIf e1 e2 e3 -> ()
+      (requires (typing e empty=Some TBool /\ is_value e))
+      (ensures \r -> is_ETrue e \/ is_EFalse e)
+let canonical_forms_bool e = ()
 
 val canonical_forms_fun : e:exp -> t1:ty -> t2:ty -> Pure unit
-      (requires ((typing e empty = Some (TArrow t1 t2)) /\ (is_value e = true)))
+      (requires (typing e empty = Some (TArrow t1 t2) /\ is_value e))
       (ensures \r -> (is_EAbs e))
 let canonical_forms_fun e t1 t2 = ()
 
-(* "An unknown assertion in the term at this location was not provable."
-   No wonder that the first case of progress fails.
-   Logic encoding of empty looks reasonable, Z3 should be able to prove this.
-   Is the encoding of is_None broken? I wasn't able to find any equations for it.
-   Only Prims.fst and Prims.snd get equations? *)
 val sel_empty : x:int -> Fact unit
       (ensures (is_None (empty x)))
 let sel_empty x = ()
 
-(* "An unknown assertion in the term at this location was not provable."
-   The (for some reason) unprovable query looks like this:
-   (= (Prims.op_Equality (Prims.option Stlc.ty)
-                         (Stlc.empty x___844)
-                         (Prims.None Stlc.ty))
-      (BoxBool true)) *)
 val sel_empty' : x:int -> Fact unit
       (ensures (empty x = None))
 let sel_empty' x = ()
@@ -161,11 +133,6 @@ val progress : e:exp -> t:ty -> Pure unit
       (ensures \r -> (is_value e \/ (is_Some (step e))))
 let rec progress e t =
   match e with
-  | EVar x ->
-      (* assert(typing (EVar x) empty = None);
-         -- this fails and it shouldn't; the case should be trivial
-         -- spawned it off as a lemma above for further investigation *)
-      admit()
   | EApp e1 e2 -> begin
       match typing e1 empty with
       | Some (TArrow t1 t2) ->
@@ -174,7 +141,10 @@ let rec progress e t =
   | EIf e1 e2 e3 ->
       progress e1 TBool; progress e2 t; progress e3 t;
       if is_value e1 then canonical_forms_bool e1
-  | _ -> ()
+  | EVar _
+  | ETrue
+  | EFalse
+  | EAbs _ _ _ -> () (* NS: writing default cases for recursive functions is bad for the solver. TODO: fix *)
 
 val appears_free_in : x:int -> e:exp -> Tot bool
 let rec appears_free_in x e =
@@ -184,106 +154,94 @@ let rec appears_free_in x e =
   | EAbs y _ e1 -> x <> y && appears_free_in x e1
   | EIf e1 e2 e3 ->
       appears_free_in x e1 || appears_free_in x e2 || appears_free_in x e3
-  | _ -> false
+  | ETrue
+  | EFalse -> false
 
 type closed e = (forall (x:int). not (appears_free_in x e))
 
-(* Adding the rec keyword on this one makes it blow up,
-   no matter what's inside it, triggered by the function argument?
-   Filed as: https://github.com/FStarLang/FStar/issues/43 *)
-val free_in_context : x:int -> e:exp -> t:ty -> g:env -> Pure unit
-      (requires (appears_free_in x e /\ typing e g = Some t))
+val free_in_context : x:int -> e:exp -> g:env -> Pure unit
+      (requires (appears_free_in x e /\ is_Some (typing e g)))
       (ensures \r -> (is_Some (g x)))
-let (* rec *) free_in_context x e t g =
+let rec free_in_context x e g =
   match e with
-  | EAbs y _ e1 ->
-      begin
-      match typing e g with
-      | Some (TArrow t1 t2) ->
-          admit() (* free_in_context x e1 t2 (extend g y t1) *)
-      | _ -> admit() (* F* can't prove this is unreachable *)
-      end
-  | EApp e1 e2 -> begin
-      match typing e1 g with
-      | Some (TArrow t1 t2) ->
-          if appears_free_in x e1 then
-            admit() (* free_in_context x e1 (TArrow t1 t2) *)
-          else
-            admit() (* free_in_context x e2 t1 *)
-      end
-  | EIf e1 e2 e3 -> begin
-      if appears_free_in x e1 then
-        admit() (* free_in_context x e1 TBool *)
-      else if appears_free_in x e2 then
-        admit() (* free_in_context x e2 t *)
-      else
-        admit() (* free_in_context x e3 t *)
-      end
+  | EAbs y t e1 -> 
+     if x = y 
+     then ()
+     else free_in_context x e1 (extend g y t)
+
+  | EApp e1 e2 -> 
+     if appears_free_in x e1
+     then free_in_context x e1 g
+     else free_in_context x e2 g
+
+  | EIf e1 e2 e3 -> 
+     if      appears_free_in x e1 then free_in_context x e1 g
+     else if appears_free_in x e2 then free_in_context x e2 g
+     else                              free_in_context x e3 g
+
   | _ -> ()
 
 (* Corollary of free_in_context *)
-val typable_empty_closed : x:int -> e:exp -> Pure unit
-      (requires (is_Some (typing e empty)))
-      (ensures \r -> closed e)
-let typable_empty_closed x e =
-  match typing e empty with
-  | Some t -> admit() (* free_in_context x e t empty -- this blows up
-                         Filed as: https://github.com/FStarLang/FStar/issues/46 *)
+val typable_empty_closed : x:int -> e:exp -> Lemma
+      (requires (is_Some (typing e empty) /\ appears_free_in x e))
+      (ensures False)
+      ([VPat (is_Some (typing e empty)); 
+        VPat (appears_free_in x e)])
+let typable_empty_closed x e = free_in_context x e empty
 
-val context_invariance : g:env -> g':env -> e:exp -> t:ty -> Pure unit
+val context_invariance : e:exp -> t:ty -> g:env -> g':env -> Pure unit
       (requires (typing e g = Some t /\
                 (forall (x:int). appears_free_in x e ==> g x = g' x)))
       (ensures \r -> (typing e g' = Some t))
-let rec context_invariance g g' e t =
+let rec context_invariance e t g g' =
   match e with
-  | EAbs x t e1 -> begin
-      (* bogus incomplete patterns error,
-         even when I do write the None pattern,
-         (I shouldn't have to, because that's unreachable anyway)
-         + equaly bogus bad postcondition error, both branches are admitted!
-         Simplified and filed as: https://github.com/FStarLang/FStar/issues/44
-         and https://github.com/FStarLang/FStar/issues/45 *)
-      match typing e1 (extend g x t) with
-      | Some t' ->
-          context_invariance (extend g x t) (extend g' x t) e1 t';
-          admit()
-      | None -> admit()
-      end
-  | EApp e1 e2 -> begin
-      match typing e1 g with
-      | Some (TArrow t1 t2) ->
-          context_invariance g g' e1 (TArrow t1 t2);
-          context_invariance g g' e2 t1
-      end
+  | EAbs x t e1 -> 
+     let (Some t') = typing e1 (extend g x t) in
+     context_invariance e1 t' (extend g x t) (extend g' x t) 
+
+  | EApp e1 e2 -> 
+     let (Some (TArrow t1 t2)) = typing e1 g in
+     context_invariance e1 (TArrow t1 t2) g g';
+     context_invariance e2 t1 g g'
+
   | EIf e1 e2 e3 ->
-      context_invariance g g' e1 TBool;
-      context_invariance g g' e2 t;
-      context_invariance g g' e3 t
+     context_invariance e1 TBool g g';
+     context_invariance e2 t g g';
+     context_invariance e3 t g g'
+
   | _ -> ()
 
 (* This is a complete disaster, the typing e (extend g x u) = Some t
    assumption seems to be not usable at all in the proof *)
 val substitution_preserves_typing :
-      g:env -> x:int -> e:exp -> u:ty -> t:ty -> v:exp -> Pure unit
+      x:int -> e:exp -> u:ty -> t:ty -> v:exp -> g:env -> Pure unit
           (requires (typing e (extend g x u) = Some t /\
                      typing v empty = Some u))
           (ensures \r -> (typing (subst x v e) g = Some t))
-let substitution_preserves_typing g x e u t v =
-  typable_empty_closed x v;
+let substitution_preserves_typing x e u t v g  =
+  (* typable_empty_closed x v; *)
   match e with
-  | EVar x' -> (* (subst x v e) = if x = x' then e else e' *)
-      (* assert(typing e (extend g x u) = (extend g x u) x);
-           -- this should work but it fails (just unfolding definition) *)
-      if x = x' then begin
-        extend_eq g x u;
-        assert(x = x'); assert(e = EVar x);
-        (* assert(u = t);  -- this should work but it fails *)
-        admit()
-      end else begin
-        assert(x<>x');
-        extend_neq g x u x';
-        admit()
-      end
+  | EVar x' -> 
+     if x'=x
+     then begin
+         assert (forall (y:int). appears_free_in y v ==> (empty y = g y));
+         admit()
+//       context_invariance v t empty g
+       end
+     else admit()
+     (* (\* (subst x v e) = if x = x' then e else e' *\) *)
+     (*  (\* assert(typing e (extend g x u) = (extend g x u) x); *)
+     (*       -- this should work but it fails (just unfolding definition) *\) *)
+     (*  if x = x' then begin *)
+     (*    extend_eq g x u; *)
+     (*    assert(x = x'); assert(e = EVar x); *)
+     (*    (\* assert(u = t);  -- this should work but it fails *\) *)
+     (*    admit() *)
+     (*  end else begin *)
+     (*    assert(x<>x'); *)
+     (*    extend_neq g x u x'; *)
+     (*    admit() *)
+     (*  end *)
   | EAbs x' t e1 ->
       admit() (* EAbs x t (if x = x' then e1 else (subst x e e1)) *)
   | EApp e1 e2 ->
@@ -296,43 +254,43 @@ let substitution_preserves_typing g x e u t v =
   | EIf e1 e2 e3 ->
       admit() (* EIf (subst x e e1) (subst x e e2) (subst x e e3) *)
 
-val preservation : e:exp -> e':exp -> t:ty -> Pure unit
-      (requires (typing e empty = Some t /\ step e = Some e'))
-      (ensures \r -> (typing e' empty = Some t))
-let rec preservation e e' t =
-  match e with
-  | EApp e1 e2 -> begin
-      match typing e1 empty with
-      | Some (TArrow t1 t2) -> begin
-          assert(typing e2 empty = Some t1); (* -- works *)
-          assert(typing e empty = Some t2); (* -- works *)
-          if is_value e1 then
-            if is_value e2 then
-              match e1 with
-              | EAbs x t e' ->
-                  assert(step e = Some (subst x e2 e')); (* -- works *)
-(*                  assert (t = t1); -- this should work, but it doesn't *)
-(*                  assert(typing e' (extend empty x t1) = Some t2);
-                      -- this should work, but it doesn't *)
-(*                  substitution_preserves_typing empty x e' t1 t2 e2
-                      -- this should work, but now precondition fails *)
-                  admit()
-            else
-              match (step e2) with
-              | Some e2' -> preservation e2 e2' t1
-          else
-            match (step e1) with
-            | Some e1' -> preservation e1 e1' (TArrow t1 t2)
-          end
-      end
-  | EIf e1 _ _ ->
-      if is_value e1 then ()
-      else begin
-        match (step e1) with
-        | Some e1' -> preservation e1 e1' TBool
-      end
-  | _ -> ()
+(* val preservation : e:exp -> e':exp -> t:ty -> Pure unit *)
+(*       (requires (typing e empty = Some t /\ step e = Some e')) *)
+(*       (ensures \r -> (typing e' empty = Some t)) *)
+(* let rec preservation e e' t = *)
+(*   match e with *)
+(*   | EApp e1 e2 -> begin *)
+(*       match typing e1 empty with *)
+(*       | Some (TArrow t1 t2) -> begin *)
+(*           assert(typing e2 empty = Some t1); (\* -- works *\) *)
+(*           assert(typing e empty = Some t2); (\* -- works *\) *)
+(*           if is_value e1 then *)
+(*             if is_value e2 then *)
+(*               match e1 with *)
+(*               | EAbs x t e' -> *)
+(*                   assert(step e = Some (subst x e2 e')); (\* -- works *\) *)
+(* (\*                  assert (t = t1); -- this should work, but it doesn't *\) *)
+(* (\*                  assert(typing e' (extend empty x t1) = Some t2); *)
+(*                       -- this should work, but it doesn't *\) *)
+(* (\*                  substitution_preserves_typing empty x e' t1 t2 e2 *)
+(*                       -- this should work, but now precondition fails *\) *)
+(*                   admit() *)
+(*             else *)
+(*               match (step e2) with *)
+(*               | Some e2' -> preservation e2 e2' t1 *)
+(*           else *)
+(*             match (step e1) with *)
+(*             | Some e1' -> preservation e1 e1' (TArrow t1 t2) *)
+(*           end *)
+(*       end *)
+(*   | EIf e1 _ _ -> *)
+(*       if is_value e1 then () *)
+(*       else begin *)
+(*         match (step e1) with *)
+(*         | Some e1' -> preservation e1 e1' TBool *)
+(*       end *)
+(*   | _ -> () *)
 
-(* CH: With this purely-executable way of specifying things we can't
-   do rule induction, and that is restrictive and will probably lead
-   to rather unnatural proofs. *)
+(* (\* CH: With this purely-executable way of specifying things we can't *)
+(*    do rule induction, and that is restrictive and will probably lead *)
+(*    to rather unnatural proofs. *\) *)
